Removed id and client from request response pairs

src/lib/communication/DY.Lib.Communication.Properties.fst
@@ -6,6 +6,7 @@ open DY.Lib.Crypto.PkEncryption.Split
 open DY.Lib.Crypto.Signature.Split
 open DY.Lib.Event.Typed
 open DY.Lib.State.PKI
+open DY.Lib.State.PrivateKeys
 open DY.Lib.State.Typed
 
 open DY.Lib.Communication.Core
@@ -17,39 +18,49 @@ open DY.Lib.Communication.RequestResponse.Invariants
 
 #set-options "--fuel 0 --ifuel 0 --z3rlimit 10 --z3cliopt 'smt.qi.eager_threshold=100'"
 
-/// This module contains experimental functions
-/// that extract properties from the communication
-/// API and make them available to a higher layer.
-/// It is not used currently and does probably not
-/// give meaning full properties.
+/// This module contains security properties that can be proven from the
+/// communication layer guarantees.
 
-val confidential_message_send:
-  {|crypto_invariants|} ->
-  tr:trace ->
-  payload:bytes -> prop
-let confidential_message_send tr payload =
-  exists i pk nonce.
-    let msg = encrypt_message payload pk nonce in
-    event_at tr i (MsgSent msg) /\
-    bytes_invariant tr msg
+(*** Authenticated Messages Properties ***)
 
-val confidential_message_sender_authentication:
-  {|invs:protocol_invariants|} ->
-  tr:trace ->
+val sender_authentication:
+  {|protocol_invariants|} ->
+  tr:trace -> i:timestamp ->
   higher_layer_preds:comm_higher_layer_event_preds ->
-  receiver:principal ->
+  sender:principal -> receiver:principal ->
   payload:bytes ->
   Lemma
   (requires
-    trace_invariant tr  /\
+    trace_invariant tr /\
     has_communication_layer_event_predicates higher_layer_preds /\
-    event_triggered tr receiver (CommConfReceiveMsg receiver payload)
+    event_triggered_at tr i receiver (CommAuthReceiveMsg sender receiver payload)
   )
   (ensures
-    (exists sender. event_triggered tr sender (CommConfSendMsg sender receiver payload)) \/
-    is_publishable tr payload
+    event_triggered (prefix tr i) sender (CommAuthSendMsg sender payload) \/
+    is_corrupt (prefix tr i) (long_term_key_label sender)
   )
-let confidential_message_sender_authentication #invs tr hlp receiver payload = ()
+let sender_authentication tr i higher_layer_preds sender receiver secret = ()
+
+
+(*** Confidential and Authenticated Messages Properties ***)
+
+val sender_confauth_authentication:
+  {|protocol_invariants|} ->
+  tr:trace -> i:timestamp ->
+  higher_layer_preds:comm_higher_layer_event_preds ->
+  sender:principal -> receiver:principal ->
+  payload:bytes ->
+  Lemma
+  (requires
+    trace_invariant tr /\
+    has_communication_layer_event_predicates higher_layer_preds /\
+    event_triggered_at tr i receiver (CommConfAuthReceiveMsg sender receiver payload)
+  )
+  (ensures
+    event_triggered tr sender (CommConfAuthSendMsg sender receiver payload) \/
+    is_corrupt tr (long_term_key_label sender)
+  )
+let sender_confauth_authentication tr i higher_layer_preds sender receiver secret = ()
 
 
 (*** Request Response Pair Properties ***)
@@ -58,37 +69,38 @@ val server_authentication:
   {|protocol_invariants|} ->
   tr:trace -> i:timestamp ->
   higher_layer_resreq_preds:comm_reqres_higher_layer_event_preds ->
-  client:principal -> server:principal -> id:bytes -> payload:bytes -> key:bytes ->
+  client:principal -> server:principal -> payload:bytes -> key:bytes ->
   Lemma
   (requires
     trace_invariant tr /\
     has_communication_layer_reqres_event_predicates request_response_event_preconditions higher_layer_resreq_preds /\
-    event_triggered_at tr i client (CommClientReceiveResponse client server  id payload key)    
+    event_triggered_at tr i client (CommClientReceiveResponse client server  payload key)    
   )
   (ensures
-    event_triggered (prefix tr i) server (CommServerSendResponse server id payload) \/
+    event_triggered (prefix tr i) server (CommServerSendResponse server payload) \/
     is_corrupt (prefix tr i) (principal_label client) \/ 
     is_corrupt (prefix tr i) (principal_label server)
   )
-let server_authentication #invs tr i higher_layer_resreq_preds client server id payload key = ()
+let server_authentication #invs tr i higher_layer_resreq_preds client server payload key = ()
 
 val key_secrecy_client:
   {|protocol_invariants|} ->
   tr:trace ->
   client:principal -> server:principal ->
-  id:bytes -> key:bytes -> payload:bytes -> 
+  key:bytes -> payload:bytes -> 
   Lemma
   (requires
     trace_invariant tr /\
     has_communication_layer_state_predicates /\
     attacker_knows tr key /\
     (
-      (exists sid. state_was_set tr client sid (ClientSendRequest {id; server; payload; key})) \/
-      (exists sid. state_was_set tr client sid (ClientReceiveResponse {id; server; payload; key}))
+      (exists sid. state_was_set tr client sid (ClientSendRequest {server; payload; key})) \/
+      (exists sid. state_was_set tr client sid (ClientReceiveResponse {server; payload; key}))
     )
   )
   (ensures
     is_corrupt tr (principal_label client) \/ is_corrupt tr (principal_label server)
   )
-let key_secrecy_client tr client server id key payload =
-  attacker_only_knows_publishable_values tr key
+let key_secrecy_client tr client server key payload =
+  attacker_only_knows_publishable_values tr key;
+  ()
